Rename vo and pc to val_obs and proph_ctrl

nola/iris/proph_ag.v
@@ -24,38 +24,40 @@ Section proph_ag.
   Context `{!proph_agG TY Σ, !prophGS TY Σ}.
 
   (** Value observer *)
-  Definition vo γ X x : iProp Σ := (ghost_var γ (1/2) (Anyty X x)).
+  Definition val_obs γ X x : iProp Σ := ghost_var γ (1/2) (Anyty X x).
   (** Double value observer *)
-  Definition vo2 γ X x : iProp Σ := (ghost_var γ 1 (Anyty X x)).
+  Definition val_obs2 γ X x : iProp Σ := ghost_var γ 1 (Anyty X x).
   (** Prophecy controller *)
-  Definition pc γ X x (ξ : prvar X) : iProp Σ :=
-    (vo γ X x ∗ 1:[ξ]) ∨
-    ((∃ x', vo2 γ X x') ∗ ⟨π, π ξ = x⟩).
+  Definition proph_ctrl γ X x (ξ : prvar X) : iProp Σ :=
+    (val_obs γ X x ∗ 1:[ξ]) ∨
+    ((∃ x', val_obs2 γ X x') ∗ ⟨π, π ξ = x⟩).
 
-  (** [vo] and [vo2] can't coexist *)
-  Lemma vo_vo2 {γ X x x'} : vo γ X x -∗ vo2 γ X x' -∗ False.
+  (** [val_obs] and [val_obs2] can't coexist *)
+  Lemma vo_vo2 {γ X x x'} : val_obs γ X x -∗ val_obs2 γ X x' -∗ False.
   Proof.
     iIntros "vo vo'". by iDestruct (ghost_var_valid_2 with "vo vo'") as %[? _].
   Qed.
 
-  (** Allocate [vo] and [pc] *)
-  Lemma vo_pc_alloc {X x} {ξ : prvar X} : 1:[ξ] ==∗ ∃ γ, vo γ X x ∗ pc γ X x ξ.
+  (** Allocate [val_obs] and [proph_ctrl] *)
+  Lemma vo_pc_alloc {X x} {ξ : prvar X} :
+    1:[ξ] ==∗ ∃ γ, val_obs γ X x ∗ proph_ctrl γ X x ξ.
   Proof.
     iIntros "ξ". iMod ghost_var_alloc as (γ) "[vo vo']". iModIntro. iExists _.
     iFrame "vo". iLeft. iFrame.
   Qed.
 
-  (** Agreement between [vo] and [pc] *)
-  Lemma vo_pc_agree {γ X x x' ξ} : vo γ X x -∗ pc γ X x' ξ -∗ ⌜x = x'⌝.
+  (** Agreement between [val_obs] and [proph_ctrl] *)
+  Lemma vo_pc_agree {γ X x x' ξ} :
+    val_obs γ X x -∗ proph_ctrl γ X x' ξ -∗ ⌜x = x'⌝.
   Proof.
     iIntros "vo [[vo' _]|[[% vo2] _]]"; last first.
     { iDestruct (vo_vo2 with "vo vo2") as %[]. }
     iDestruct (ghost_var_agree with "vo vo'") as %?. by simplify_eq.
   Qed.
 
-  (** Update the value of [vo] and [pc] *)
+  (** Update the value of [val_obs] and [proph_ctrl] *)
   Lemma vo_pc_update {γ X x x' y ξ} :
-    vo γ X x -∗ pc γ X x' ξ ==∗ vo γ X y ∗ pc γ X y ξ.
+    val_obs γ X x -∗ proph_ctrl γ X x' ξ ==∗ val_obs γ X y ∗ proph_ctrl γ X y ξ.
   Proof.
     iIntros "vo [[vo' ξ]|[[% vo2] _]]"; last first.
     { iDestruct (vo_vo2 with "vo vo2") as %[]. }
@@ -63,10 +65,11 @@ Section proph_ag.
     iModIntro. iLeft. iFrame.
   Qed.
 
-  (** Resolve the prophecy of [pc] *)
+  (** Resolve the prophecy of [proph_ctrl] with [val_obs],
+    retaining [proph_ctrl] *)
   Lemma vo_pc_preresolve {γ X x x'} ξ aπ ηl q : aπ ./ ηl →
-    q:∗[ηl] -∗ vo γ X x -∗ pc γ X x' ξ =[proph_wsat]=∗
-      q:∗[ηl] ∗ ⟨π, π ξ = aπ π⟩ ∗ (∀ y, ⟨π, aπ π = y⟩ -∗ pc γ X y ξ).
+    q:∗[ηl] -∗ val_obs γ X x -∗ proph_ctrl γ X x' ξ =[proph_wsat]=∗
+      q:∗[ηl] ∗ ⟨π, π ξ = aπ π⟩ ∗ (∀ y, ⟨π, aπ π = y⟩ -∗ proph_ctrl γ X y ξ).
   Proof.
     iIntros "% ηl vo [[vo' ξ]|[[% vo2] _]]"; last first.
     { iDestruct (vo_vo2 with "vo vo2") as %[]. }
@@ -74,9 +77,9 @@ Section proph_ag.
     iFrame "obs". iIntros "%y obs'". iRight. iCombine "vo vo'" as "vo2".
     iSplit; [by iExists _|]. by iApply (proph_obs_impl2 with "obs obs'")=> ?->.
   Qed.
+
+  (** Resolve the prophecy of [proph_ctrl] *)
   Lemma pc_resolve {γ X x} ξ :
-    pc γ X x ξ =[proph_wsat]=∗ ⟨π, π ξ = x⟩.
-  Proof.
-    iIntros "[[_ ξ]|[_ $]]"; [|done]. iApply (proph_resolve with "ξ").
-  Qed.
+    proph_ctrl γ X x ξ =[proph_wsat]=∗ ⟨π, π ξ = x⟩.
+  Proof. iIntros "[[_ ξ]|[_ $]]"; [|done]. iApply (proph_resolve with "ξ"). Qed.
 End proph_ag.
